\section{Trace equivalence}

Let $\alpha(\iota, k) \triangleq \alpha \text{ s. t. } \alpha \in \{ \actread{\iota}{k}{v}, \actwrite{\iota}{k}{v}\ |\ v \in \mathsf{Val} \}$

\lem
\begin{gather*}
	\forall h, h', \Phi, \Phi', S, S', \mathds{P}, \mathds{P}', i, j, k, k', v, v' \ldotp \\
	 i \neq j \implies
	 \\
	(\exists h_0, \Phi_0, S_0, \mathds{P}_0 \ldotp 
	(h, \Phi, S, \mathds{P}) \xrightarrow{\actread{i}{k}{v}} (h_0, \Phi_0, S_0, \mathds{P}_0)  \xrightarrow{\actread{j}{k'}{v'}} (h', \Phi', S', \mathds{P}') \\
	\iff \\
	\exists h_1, \Phi_1, S_1, \mathds{P}_1 \ldotp
	(h, \Phi, S, \mathds{P}) \xrightarrow{\actread{j}{k'}{v'}} (h_1, \Phi_1, S_1, \mathds{P}_1) \xrightarrow{\actread{i}{k}{v}} (h', \Phi', S', \mathds{P}'))
\end{gather*}

\lem
\begin{gather*}
	\forall h, h', \Phi, \Phi', S, S', \mathds{P}, \mathds{P}', i, j, k, k', x, y \ldotp \\
	x = \alpha(i, k) \land y = \alpha(j, k') \implies \\
	(\exists h_0, \Phi_0, S_0, \mathds{P}_0 \ldotp
	(h, \Phi, S, \mathds{P}) \xrightarrow{x} (h_0, \Phi_0, S_0, \mathds{P}_0)  \xrightarrow{y} (h', \Phi', S', \mathds{P}') \land i \neq j \land k \neq k' \\
	\iff \\
	\exists h_1, \Phi_1, S_1, \mathds{P}_1 \ldotp
	(h, \Phi, S, \mathds{P}) \xrightarrow{y} (h_1, \Phi_1, S_1, \mathds{P}_1) \xrightarrow{x} (h', \Phi', S', \mathds{P}'))
\end{gather*}

\lem
\begin{gather*}
	\forall h, h', \Phi, \Phi', S, S', \mathds{P}, \mathds{P}', i, j, n, n', l, l' \ldotp \\
	i \neq j \implies \\
	(\exists h_0, \Phi_0, S_0, \mathds{P}_0 \ldotp 
	(h, \Phi, S, \mathds{P}) \xrightarrow{\actalloc{i}{n}{l}} (h_0, \Phi_0, S_0, \mathds{P}_0)  \xrightarrow{\actalloc{j}{n'}{l'}} (h', \Phi', S', \mathds{P}') \\
	\iff \\
	\exists h_1, \Phi_1, S_1, \mathds{P}_1 \ldotp
	(h, \Phi, S, \mathds{P}) \xrightarrow{\actalloc{j}{n'}{l'}} (h_1, \Phi_1, S_1, \mathds{P}_1) \xrightarrow{\actalloc{i}{n}{l}} (h', \Phi', S', \mathds{P}'))
\end{gather*}

\lem
\begin{gather*}
	\forall h, h', \Phi, \Phi', S, S', \mathds{P}, \mathds{P}', i, j, n, l, k, x \ldotp \\
	x = \alpha(j, k) \land i \neq j \land (k < l \lor k \geq l + n) \implies \\
	(\exists h_0, \Phi_0, S_0, \mathds{P}_0 \ldotp 
	(h, \Phi, S, \mathds{P}) \xrightarrow{\actalloc{i}{n}{l}} (h_0, \Phi_0, S_0, \mathds{P}_0)  \xrightarrow{x} (h', \Phi', S', \mathds{P}') \\
	\iff \\
	\exists h_1, \Phi_1, S_1, \mathds{P}_1 \ldotp
	(h, \Phi, S, \mathds{P}) \xrightarrow{x} (h_1, \Phi_1, S_1, \mathds{P}_1) \xrightarrow{\actalloc{i}{n}{l}} (h', \Phi', S', \mathds{P}'))
\end{gather*}
